Added more Gen and Show instances for local BC

execution/theories/Generators.v
@@ -5,7 +5,7 @@ From ExtLib.Structures Require Import Functor Applicative.
 From ConCert Require Import Blockchain.
 From ConCert Require Import LocalBlockchain.
 From ConCert Require Import Serializable.
-From ConCert Require Import BoundedN.
+From ConCert Require Import BoundedN ChainedList.
 (* For monad notations *)
 Require Export ExtLib.Structures.Monads.
 Export MonadNotation. Open Scope monad_scope.
@@ -14,28 +14,45 @@ From Coq Require Import List.
 From Coq Require Import Strings.BinaryString.
 Import ListNotations.
 
-(* Module DoNotation.
-Import ssrfun.
-Notation "'do!' X <- A ; B" :=
-  (bindGen A (fun X => B))
-  (at level 200, X ident, A at level 100, B at level 200).
-End DoNotation.
-Import DoNotation. *)
-
 (* Declare Instance genAmountSized : GenSized Amount.
 Declare Instance showAmount : Show Amount.
 Declare Instance shrinkAmount : Shrink Amount. *)
 
 
-Instance showAmount : Show Amount :=
+Record BaseGens (BaseTypes : ChainBase) := 
+  mkBaseGens {
+    (* Address          : Type; *)
+    gAddress              : G (@Address BaseTypes);
+    init_account_balances : @Address BaseTypes -> Amount;
+    gValidContractAddr    : G (@Address BaseTypes);
+    (* genSetup         : G Setup;
+    genMsg           : G Msg;
+    genState         : G State;
+    genSerializedVal : G SerializedValue; *)
+  }.
+  
+Open Scope string_scope.
+Instance showBaseGens {BaseTypes : ChainBase} : Show (BaseGens BaseTypes)  :=
   {|
-    show := @show Z showZ
+    show bg := "BaseGens{...}"
   |}.
 
-Instance genAmountSized : GenSized Amount :=
+(* Instance showAmount : Show Amount :=
+  {|
+    show := @show Z showZ
+  |}. *)
+
+
+(* Instance genAmountSized : GenSized Amount :=
   {|
     arbitrarySized := @arbitrarySized Z _ 
   |}.
+
+Instance genAmount : Gen Amount :=
+  {|
+    arbitrary := @arbitrary Z _ 
+  |}. *)
+
 
 Instance shrinkAmount : Shrink Amount := 
   {|
@@ -43,73 +60,63 @@ Instance shrinkAmount : Shrink Amount :=
   |}.
 
   
-(* dummy implementation for now *)
+(* dummy implementations for now *)
 Definition empty_str : string := "".
 Definition sep : string := ", ".
 
 
-
-Record BaseGens {Setup Msg State : Type} := 
-  mkBaseGens {
-    (* Address          : Type; *)
-    genAddress       : G Blockchain.Address;
-    genSetup         : G Setup;
-    genMsg           : G Msg;
-    genState         : G State;
-    genSerializedVal : G SerializedValue;
-  }.
-
-
-Open Scope string_scope.
 Instance showChain (BaseTypes : ChainBase) : Show (@Chain BaseTypes) :=
   {|
     show c := 
       let height := show (chain_height c) in
       let slot := show (current_slot c) in
       let fin_height := show (finalized_height c) in
-        "{" ++ height ++ sep ++ slot ++ sep ++ fin_height ++ "}"
+        "Chain{" ++ "height: " ++ height ++ sep 
+                 ++ "current slot: " ++ slot ++ sep 
+                 ++ "final height: " ++ fin_height 
+                 ++ "}"
+  |}.
+
+
+Instance showEnvironment (BaseTypes : ChainBase) `{Show Chain}: Show Environment :=
+  {|
+    show env := "Environment{" 
+                ++ "chain: " ++ show (env_chain env) ++ sep 
+                ++ "contract states: ..."
+                ++ "}"
   |}.
 
 Close Scope string_scope.
 
+Open Scope list_scope.
 
-
-Fixpoint mkMapFromList {B : Type}
-                       (address_eqb : Address -> Address -> bool)
-                       (genB : G B)
-                       (l : list Address) 
-                       : G (Address -> B) :=
-  match l with
-  | [] => b <- genB ;; returnGen (fun x => b)
-  | a::l' =>
-    b <- genB ;;
-    liftM 
-      (fun (mp : Address -> B) (x : Address) 
-        => if address_eqb x a then b else mp x) 
-      (mkMapFromList address_eqb genB l')
+Fixpoint mkMapFromList {A B : Type}
+                       (a_eqb : A -> A -> bool)
+                       (default : B)
+                       (l : list A) 
+                       (lb : list B)
+                       : A -> B :=
+  match (l,lb) with
+  | ([],[]) => fun x => default
+  | (a::l', b::lb') => 
+    fun (x : A) => if a_eqb x a then b else (mkMapFromList a_eqb default l' lb') x 
+  | (_,_) => fun x => default
   end.
 
-Definition mkMapFromListGen {B : Type}
-                          (address_eqb : Address -> Address -> bool)
-                          (genB : G B)
-                          (genListA : G (list Address)) 
-                          : G (Address -> B) :=
-  listA <- genListA ;; mkMapFromList address_eqb genB listA.
 
 (* Makes a generator for BlockChains, given generators for the necessary types: Address, Setup, Msg, State, SerializedValue. 
    Ensures that all address usages are consistent with the generated address mapping. *)
-Definition mkChainGen {Setup Msg State : Type}
-                        (baseGens : @BaseGens Setup Msg State) (BaseTypes : ChainBase)
-                        : nat -> G (@Chain BaseTypes)  := 
-  fun n =>
+Definition mkChainGen (BaseTypes : ChainBase) (baseGens : BaseGens BaseTypes) (n : nat)
+                      : G Chain  := 
   (* First construct context of Contract Addresses. *)
-  let g_address := genAddress baseGens in
-  let addr_eqb : Address -> Address -> bool := address_eqb in
-  let addr_list_gen : G (list Blockchain.Address) := vectorOf n g_address in
     ch_height  <- arbitrarySized n ;;
     cur_slot   <- arbitrarySized ch_height ;; (* We make sure current slot is <= chain height *)
-    mp         <- mkMapFromListGen addr_eqb (sized arbitrarySized) addr_list_gen ;; 
-    returnGen (build_chain ch_height cur_slot n (fun (a : Blockchain.Address) => Z.of_nat n)).
+    (* gmp         <- liftM (mkMapFromList addr_eqb (arbitrarySized n)) addr_list_gen ;; 
+    mp <- gmp ;; *)
+    let acc_bal := init_account_balances BaseTypes baseGens in
+    returnGen (build_chain ch_height cur_slot n acc_bal).
+    
+Close Scope list_scope.
 
   (* For now, shrinking does nothing *)
 Instance shrinkChain (BaseTypes : ChainBase) : Shrink (@Chain BaseTypes) :=
@@ -117,16 +124,67 @@ Instance shrinkChain (BaseTypes : ChainBase) : Shrink (@Chain BaseTypes) :=
     shrink c := cons c nil
   |}.
 
+Derive Arbitrary for SerializedType.
+Derive Show for SerializedType.
+Import SerializedType.
+Open Scope list_scope.
+Open Scope string_scope.
 
+Fixpoint string_of_interp_type (st : SerializedType) :  (interp_type st) -> string :=
+match st as st0 return interp_type st0 -> string with
+  | ser_unit => fun _ => "()"
+  | ser_int => fun t => show t
+  | ser_bool => fun t => show t
+  | ser_list a => 
+    fun t : list (interp_type a) => 
+      let t_str_list := map (string_of_interp_type a) t in 
+      "[" ++ String.concat ";" t_str_list ++ "]"  
+  | ser_pair a b => 
+    fun t : (interp_type a * interp_type b) => 
+      "(" 
+      ++ string_of_interp_type a (fst t) 
+      ++ ","
+      ++ string_of_interp_type b (snd t) ++ ")"
+  end.  
 
-Module LocalBlockchainGens.
+Definition ex_serialized_type := ser_pair (ser_list (ser_list ser_bool)) ser_int.
+Compute (interp_type ex_serialized_type).
+Definition ex_val := ([[true;false];[true;true];[false];[]], 2%Z).
+Compute (string_of_interp_type ex_serialized_type ex_val).
+
+Close Scope list_scope.
+Instance showSerializedValue : Show SerializedValue := 
+  {|
+    show v := "SerializedValue{" 
+              ++ show (ser_value_type v) ++ sep
+              ++ string_of_interp_type (ser_value_type v) (ser_value v) ++ "}" 
+  |}.
+Close Scope string_scope.
+
+Fixpoint gInterp_type (t : SerializedType) : G (interp_type t) := 
+  match t with
+  | ser_unit => returnGen tt
+  | ser_int => @arbitrary Z _
+  | ser_bool => arbitrary
+  | ser_pair a b => liftM2 pair (gInterp_type a) (gInterp_type b) 
+  | ser_list a => listOf (gInterp_type a)
+  end.
+
+Definition gSerializedValueSized (n : nat): G SerializedValue :=
+  t <- arbitrarySized n ;;
+  liftM (build_ser_value t) (gInterp_type t).
+
+Instance genSerializedValueSized : GenSized SerializedValue :=
+  {|
+    arbitrarySized := gSerializedValueSized 
+  |}.
+
+(* Sample (@arbitrarySized SerializedType _ 3). *)
+(* Sample (@arbitrarySized SerializedValue _ 3). *)
 
 Import BoundedN.Stdpp.
-Global Opaque Address. 
-
-Print LocalChainBase.
-
-Definition b10 : Address := BoundedN.of_Z_const AddrSize 10.
+Import LocalBlockchain.
+Definition zero_address : Address := BoundedN.of_Z_const AddrSize 10.
 Definition b9 : option (BoundedN.BoundedN AddrSize) := @BoundedN.of_nat AddrSize 9.
 
 
@@ -151,11 +209,19 @@ Instance showBoundedNAddrSize : Show (BoundedN.BoundedN AddrSize) :=
     show := @show (BoundedN.BoundedN AddrSize) showBoundedN
   |}.
 
-Instance showAddress : Show Address :=
+Instance showAddress : Show (@Address LocalChainBase) :=
   {|
     show := @show (BoundedN.BoundedN AddrSize) showBoundedN
   |}.
 
+Instance showLocalChain : Show LocalChain := 
+  {|
+    show lc := "LocalChain{" 
+                ++ show (lc_height lc) ++ sep 
+                ++ show (lc_slot lc)   ++ sep 
+                ++ show (lc_fin_height lc) 
+                ++ sep ++ "... }"
+  |}.
 
 
 Close Scope string_scope.
@@ -169,13 +235,13 @@ Derive Arbitrary for positive.
 Derive GenSized for positive.
 
 (* Although the type is G (option ...) it will never generate None values *)
-Definition genBoundedNOpt (bound : N): G (option (BoundedN.BoundedN bound)) :=
+Definition gBoundedNOpt (bound : N): G (option (BoundedN.BoundedN bound)) :=
   n <- arbitrarySized (N.to_nat bound) ;; (* we exploit that arbitrarySized n on nats automatically bounds the value by <= n *)
   returnGen (@decode_bounded bound (Pos.of_nat n)).
 
 
-Definition genBoundedN : G (BoundedN.BoundedN AddrSize) :=
-  bn <- genBoundedNOpt AddrSize ;;
+Definition gBoundedN : G (BoundedN.BoundedN AddrSize) :=
+  bn <- gBoundedNOpt AddrSize ;;
   returnGen match bn with
     | Some b => b
     (** The None case should never happen since 'arbitrarySized' on AddrSize already ensures that
@@ -183,40 +249,83 @@ Definition genBoundedN : G (BoundedN.BoundedN AddrSize) :=
     | None => BoundedN.of_Z_const AddrSize 0
   end. 
 
-Definition genAddress : G Address := genBoundedN.
+Instance genBoundedN : Gen (BoundedN.BoundedN AddrSize) :=
+  {|
+    arbitrary := gBoundedN
+  |}.
 
 
+Instance genAddress : Gen (@Address LocalChainBase) :=
+  {|
+    (* I could have just written 'arbitrary' here, but this is more explicit; and i like explicit code *)
+    arbitrary := @arbitrary (BoundedN.BoundedN AddrSize) genBoundedN 
+  |}.
 
-End LocalBlockchainGens.
+(* Definition genDummyChainedList : G (ChainTrace empty_state (build_chain_state lcb_lc [])) :=
+  returnGen clnil. *)
+
+Definition gDummyLocalChain : G LocalChain :=
+  returnGen lc_initial.
+
+(* always generates the initial local chain builder, which contains the initial local chain, and initial, empty trace *)
+Definition gDummyLocalChainBuilder : G LocalChainBuilder :=
+  returnGen lcb_initial.
+
+Definition gEnvFromLocalChain (lc : LocalChain) : G Environment := returnGen (lc_to_env lc) .
+
+(* Instance genEnvFromLocalChain (lc : LocalChain) : Gen Environment :=
+  {| 
+    arbitrary := gEnvFromLocalChain lc
+  |}. *)
+
+Definition gValidContractAddr' : G (@Address LocalChainBase) :=
+  n <- arbitrarySized (N.to_nat ContractAddrBase) ;; (* generates a value between 0 and ContractAddrBase (= AddrSize/2*)
+  let nn : nat := n + (N.to_nat ContractAddrBase) in (* ContractAddrBase <= nn <= AddrSize*)
+  let bound_opt : option (BoundedN.BoundedN AddrSize):= @decode_bounded AddrSize (Pos.of_nat nn) in
+  match bound_opt with
+  | Some b => returnGen b
+  | None => returnGen (BoundedN.of_Z_const AddrSize (Z.of_N ContractAddrBase)) 
+  end.
 
 
-Import LocalBlockchainGens.
+Definition gLocalBaseGens (n : nat) : G (BaseGens LocalChainBase) := 
+  let addr_eqb := @address_eqb LocalChainBase in 
+  let default : Amount := Z0 in
+  amounts    <- vectorOf n arbitrary ;;
+  addrs      <- vectorOf n arbitrary ;;
+  (* let acc_bal := fun x => default in *)
+  let acc_bal := mkMapFromList addr_eqb default addrs amounts in
+  returnGen (mkBaseGens LocalChainBase arbitrary acc_bal gValidContractAddr').
 
-Sample genAddress.
+Instance genLocalBaseGens : GenSized (BaseGens LocalChainBase) :=
+  {|
+    arbitrarySized := gLocalBaseGens
+  |}.
 
+Definition gLocalChainSized : nat -> G (@Chain LocalChainBase) := 
+  fun n => lb <- gLocalBaseGens n ;; mkChainGen LocalChainBase lb n.
 
-Sample (@arbitrarySized Chain (genChainSized LocalChainBase) 2).
-
-
-Sample (@arbitrarySized Amount _ 2).
-
-Open Scope nat_scope.
-Definition n_is_zero_nat (n : nat) := n =? 0.
-(* QuickChick n_is_zero_nat. *)
-
-
-(* Example of how to sample a specific type? *)
-Sample (@arbitrarySized Z genZSized 2).
-Sample (@arbitrarySized Amount genZSized 2).
-(* How to go from arbitrarySized to arbitrary *)
-Print sized.
-Sample (@sized Z (@arbitrarySized Z genZSized)).
-
-
-Open Scope Z_scope.
-Definition n_is_zero (n : Z) := n =? 0.
-(* QuickChick n_is_zero. *)
+  
+Instance genLocalChainSized : GenSized (@Chain LocalChainBase) :=
+{|
+  arbitrarySized := gLocalChainSized
+|}.
 
 
+Open Scope N_scope.
+Definition validcontractaddr_valid := (forAll gValidContractAddr' (fun a => (BoundedN.to_N a) <=? AddrSize)).
+(* QuickChick validcontractaddr_valid. *)
+(* Passed 10000 tests (0 discards) *)
+Close Scope N_scope.
 
+
+Open Scope list_scope.
+Definition acc_bal := mkMapFromList (fun x y => x =? y) 42 [10;20;30;40] [1;2;3;4].
+Definition testGChain : G Chain := arbitrary.
+
+
+Sample (gLocalChainSized 4).
+Sample (gLocalBaseGens 10).
+Sample (@arbitrarySized Chain _ 2).
+Sample (gEnvFromLocalChain lc_initial).
 
